
# Lon Capa 6E - Question 3 | Collisions of Point Masses in Two Dimensions

> **Question:** A *6.30* kg bowling ball moving at *9.30* m/s in the +x-axis direction collides with a *0.950* kg bowling pin, which is scattered at an angle of *80.0*Â° above the +x-axis and with a speed of *16.0* m/s. 
> 
> 1. Calculate the magnitude of the final velocity of the bowling ball.
> 2. What is the kinetic energy before the collision?
> 3. What is the kinetic energy after the collision?
> 4. Is the collision elastic? (If not, discuss how spin on the ball might be converted to linear kinetic energy in the collision.)

> m_b = 6.3 kg
> v_b = 9.3 m/s
>
> theta = 80.0 degrees
>
> m_p = 0.95 kg
> v_p = 16.0 m/s

> additionally, for further use, the angle between the x-axis and the initial velocity of the bowling ball, going counterclockwise like in the unit circle:
> 
> angle = 0.0 degrees

## Finding Momentum(s)

### The Pin:
> Finding initial momentum is easy, it is at rest, so in the equation
> p_direction = m * v * cos(theta)
> v is 0, so the entire equation = 0 N*s

p_x = 0 Ns
p_y = 0 Ns

`p_p_x_i = 0 Ns`
`p_p_y_i = 0 Ns`

> Then we need to find the final momentum in 2-D of the pin

p_x = m_p *  v_p * cos(theta)
p_y = m_p *  v_p * sin(theta)

> For my values:

p_x = 0.95 kg * 16.0 m/s * cos(80.0 degrees)
p_y = 0.95 kg * 16.0 m/s * sin(80.0 degrees)

`p_p_x_f = 2.6395 Ns`
`p_p_y_f = 14.9690 Ns`

> We'll use these later w/ conservation of momentum

### The Bowling Ball
> For the bowling ball, the initial momentum is **not** 0, so we'll calculate it to use in the equation.

> Note: You may need to amend the equation / direction if your own problem does not feature the bowling ball going in the +x-axis direction
> 
> I've used "*angle*" as the angle from the x-axis going counterclockwise, which in this case is 0. Ensure velocities are positive when using this method!

p_x = m_p * v_p * cos(angle)
p_y = m_p * v_p * sin(angle)

> For my values:

p_x = 6.3 kg * 9.3 m/s * cos(0 degrees)
p_y = 6.3 kg * 9.3 m/s * sin(0 degrees)

`p_b_x_i = 58.59 Ns`
`p_b_y_i = 0 Ns`

## Using momentum to solve
> From these values, we can use the concept of conservation of momentum to find the bowling ball's final velocity and direction

p_i = p_f

> In two dimensions, this becomes two equations:

p_x_i = p_x_f
p_y_i = p_y_f

> The net momentums are based on the combined momentums, within the context of this problem: the bowling ball and pin. Thus the equations become:

p_b_x_i + p_p_x_i = p_b_x_f + p_p_x_f
p_b_y_i + p_p_y_i = p_b_y_f + p_p_y_f

> We know the initial momentums of the ball and pin, and the final of the pin, so we can rearrange to solve for what we want, the final momentums of the ball

p_b_x_i + p_p_x_i - p_p_x_f = p_b_x_f
p_b_y_i + p_p_y_i - p_p_y_f = p_b_y_f

> or in other words

p_b_x_f = p_b_x_i + p_p_x_i - p_p_x_f
p_b_y_f = p_b_y_i + p_p_y_i - p_p_y_f

> then expand, allowing us to isolate the unknowns

v_b_x_f * m_b = p_b_x_i + p_p_x_i - p_p_x_f
v_b_y_f * m_b = p_b_y_i + p_p_y_i - p_p_y_f

v_b_x_f = (p_b_x_i + p_p_x_i - p_p_x_f) / m_b
v_b_y_f = (p_b_y_i + p_p_y_i - p_p_y_f) / m_b

> but what we really want is the magnitude of the final velocity, not its components, so we can use the Pythagorean theorem to solve for v

v_b_f = sqrt( (v_b_x_f)^2 +   (v_b_y_f)^2 )
v_b_f = sqrt( ((p_b_x_i + p_p_x_i - p_p_x_f) / m_b)^2 +  ((p_b_y_i + p_p_y_i - p_p_y_f) / m_b)^2 )

> a bit more nicely, that's

$v_{b,f}$ = $\sqrt{ (v_{b,x,f})^2 + (v_{b,y,f})^2 }$

$v_{b,f}$ = $\sqrt{ \left( \frac{p_{b,x,i} + p_{p,x,i} - p_{p,x,f}}{m_b} \right)^2 + \left( \frac{p_{b,y,i} + p_{p,y,i} - p_{p,y,f}}{m_b} \right)^2 }$

> If we really want to make this a one-line process, we can do:

$v_{b,f} = \sqrt{ \left( \frac{(m_b * v_b * cos(angle)) + 0 - (m_p *  v_p * cos(\theta))}{m_b} \right)^2 + \left( \frac{(m_b * v_b * sin(angle)) + 0 - (m_p *  v_p * sin(\theta))}{m_b} \right)^2 }$

> We can then plug in our values found in previous steps. 
> For my numbers, that would be:

$v_{b,f} =  \sqrt{ \left( \frac{(6.3\,\cdot\,9.3\,\cdot\,cos(0)) + 0 - (0.95\,\cdot\,16.0\,\cdot\,cos(80))}{6.3} \right)^2 + \left( \frac{(6.3\,\cdot\,9.3\,\cdot\,sin(0)) + 0 - (0.95\,\cdot\,16.0\,\cdot\,sin(80))}{6.3} \right)^2 }$

`v_b_f = 9.19339 m/s`

## Finding the Angle

> we can use some trig to find the angle based on the x and y components

$\sin{\theta} = \frac{opposite}{adjacent}$

$\sin{\theta} = \frac{v_{b,y,f} }{ v_{b,x,f}}$

$\theta = \sin^{-1}{\frac{v_{b,y,f} }{ v_{b,x,f}}}$

$\theta = \sin^{-1}{\frac{v_{b,y,f} }{ v_{b,x,f}}}$

> Using the equations from the previous part (which can be found in the final equations section as well):


$v_{b,x,f} = \frac{(m_b * v_b * cos(angle)) - (m_p *  v_p * cos(\theta))}{m_b}$

$v_{b,y,f} = \frac{(m_b * v_b * sin(angle)) - (m_p *  v_p * sin(\theta))}{m_b}$

> we can plug these into the equation above to get


$\theta = \sin^{-1}{\frac{\frac{(m_b\,\cdot\,v_b\,\cdot\,sin(angle)) - (m_p\,\cdot\, v_p\,\cdot\,sin(\theta))}{m_b}}{\frac{(m_b\,\cdot\,v_b\,\cdot\,cos(angle)) - (m_p\,\cdot\, v_p\,\cdot\,cos(\theta))}{m_b}}}$

> slightly more neatly that's

$\theta = \sin^{-1}{\frac{m_b\,\cdot\,v_b\,\cdot\,sin(angle) \,-\, m_p\,\cdot\, v_p\,\cdot\,sin(\theta)}{m_b\,\cdot\,v_b\,\cdot\,cos(angle) \,-\, m_p\,\cdot\, v_p\,\cdot\,cos(\theta)}}$

> for my question:

$\theta = \sin^{-1}{\frac{6.3\,\cdot\,9.3\,\cdot\,\sin(0) - 0.95\,\cdot\,16.0\,\cdot\,\sin\left(\frac{80\,\cdot\,\pi}{180}\right)}{6.3\,\cdot\,9.3\,\cdot\,\cos(0) - 0.95\,\cdot\,16.0\,\cdot\,\cos\left(\frac{80\,\cdot\,\pi}{180}\right)}}$

`theta = -14.9 deg`

## Finding Kinetic Energy (Before)
> To find net kinetic energy, we find the sum of

$K$ = $\sum{\frac{1}{2} \cdot m \cdot v^2}$

$K_i$ = $K_{b,i} + K_{p,i}$

$K_i$ = $\frac{1}{2} \cdot \left( 
m_{b} \cdot (v_{b,i})^2 + m_{p} \cdot (v_{p,i})^2
\right)$

> For my numbers:

$K_i$ = $\frac{1}{2} \cdot \left( 6.3 \cdot (9.3)^2 + 0.95 \cdot (0)^2\right)$

$K_i$ = 272.4435 J

## Finding Kinetic Energy (After)

$K_f$ = $\sum{\frac{1}{2} \cdot m \cdot v^2}$

$K_f$ = $\frac{1}{2} \cdot \left( 
m_{b} \cdot (v_{b,f})^2 + m_{p} \cdot (v_{p})^2
\right)$

> now we can substitute in that long equation for $v_{b,f}$
> the square and sqrt reduce out!

$K_f$ = $\frac{1}{2} \cdot \left( 
m_{b} \cdot \left(
 \left( \frac{(m_b\,\cdot\,v_b\,\cdot\,cos(angle)) + 0 - (m_p\,\cdot\, v_p\,\cdot\,cos(\theta))}{m_b} \right)^2 + \left( \frac{(m_b\,\cdot\,v_b\,\cdot\,sin(angle)) + 0 - (m_p\,\cdot\, v_p\,\cdot\,sin(\theta))}{m_b} \right)^2
\right) + m_{p} \cdot (v_{p})^2
\right)$

> For my numbers:

$K_i$ = $\frac{1}{2} \cdot \left( 6.3 \cdot \left(\left( \frac{(6.3\,\cdot\,9.3\,\cdot\,cos(0)) + 0 - (0.95\,\cdot\,16.0\,\cdot\,\cos{\frac{80\,\cdot\,\pi}{180}})}{6.3} \right)^2 + \left( \frac{(6.3\,\cdot\,9.3\,\cdot\,sin(0)) + 0 - (0.95\,\cdot\,16.0\,\cdot\,\sin{\frac{80\,\cdot\,\pi}{180}})}{6.3} \right)^2\right) + 0.95 \cdot (16)^2\right)$

### Is it elastic?

> Based on what we know about elasticity, the answer is the same as it would be to
> "*Was kinetic energy conserved?*"

> In my problem:
> Answer: **No**

# Final Equations
> Note: Take these with a grain of salt, it's much better to follow along with the steps in sections above, and that way you'll yk.. learn, too!


## General / Reused

> velocity (given that the pin starts at rest, otherwise follow the directions to derive again)

$v_{b,x,f} = \frac{(m_b\,\cdot\,v_b\,\cdot\,cos(angle)) - (m_p\,\cdot\, v_p\,\cdot\,cos(\theta))}{m_b}$

$v_{b,y,f} = \frac{(m_b\,\cdot\,v_b\,\cdot\,sin(angle)) - (m_p\,\cdot\, v_p\,\cdot\,sin(\theta))}{m_b}$

## Submitted
$v_{b,f} = \sqrt{ \left( \frac{(m_b\,\cdot\,v_b\,\cdot\,cos(angle)) + 0 - (m_p\,\cdot\, v_p\,\cdot\,cos(\theta))}{m_b} \right)^2 + \left( \frac{(m_b\,\cdot\,v_b\,\cdot\,sin(angle)) + 0 - (m_p\,\cdot\, v_p\,\cdot\,sin(\theta))}{m_b} \right)^2 }$

$\theta = \sin^{-1}{\frac{m_b\,\cdot\,v_b\,\cdot\,sin(angle) \,-\, m_p\,\cdot\, v_p\,\cdot\,sin(\theta)}{m_b\,\cdot\,v_b\,\cdot\,cos(angle) \,-\, m_p\,\cdot\, v_p\,\cdot\,cos(\theta)}}$

$K_i$ = $\frac{1}{2} \cdot \left( 
m_{b} \cdot (v_{b,i})^2 + m_{p} \cdot (v_{p,i})^2
\right)$

$K_f$ = $\frac{1}{2} \cdot \left( 
m_{b} \cdot \left(
 \left( \frac{(m_b\,\cdot\,v_b\,\cdot\,cos(angle)) + 0 - (m_p\,\cdot\, v_p\,\cdot\,cos(\theta))}{m_b} \right)^2 + \left( \frac{(m_b\,\cdot\,v_b\,\cdot\,sin(angle)) + 0 - (m_p\,\cdot\, v_p\,\cdot\,sin(\theta))}{m_b} \right)^2
\right) + m_{p} \cdot (v_{p})^2
\right)$